base <http://purl.org/ontology/studio/multitrack#> .
@prefix rdf: <http://www.w3.org/1999/02/22-rdf-syntax-ns#> .
@prefix mt: <http://purl.org/ontology/studio/multitrack#> .
@prefix event: <http://purl.org/NET/c4dm/event.owl#> .
@prefix owl11: <http://www.w3.org/2006/12/owl11#> .
@prefix owl11xml: <http://www.w3.org/2006/12/owl11-xml#> .
@prefix xsd: <http://www.w3.org/2001/XMLSchema#> .
@prefix mo: <http://purl.org/ontology/mo/> .
@prefix rdfs: <http://www.w3.org/2000/01/rdf-schema#> .
@prefix foaf: <http://xmlns.com/foaf/0.1/> .
@prefix owl: <http://www.w3.org/2002/07/owl#> .

<http://purl.org/ontology/studio/multitrack>
    a owl:Ontology;
    rdfs:comment "An ontology for describing concepts in multitrack media production " .

mt:MultitrackProject
    a owl:Class;
    rdfs:subClassOf foaf:Project;
    rdfs:comment "A project created in a multitrack media production tool, an audio editor, a DAW, or a sequencer of some kind." .

mt:ProjectTrack
    a owl:Class;
    rdfs:comment "A track in a multitrack project. A container type for audio/media clips, control events, feature events, or annotations." .

mt:MediaTrack
    a owl:Class;
    rdfs:subClassOf mt:ProjectTrack;
    rdfs:comment "A track in a multitrack project holding audiovisual information only. " .

mt:AudioTrack
    a owl:Class;
    rdfs:subClassOf mt:MediaTrack;
    rdfs:comment "An AudioTrack contains a set of audio clips organized in a musically meaningful way." .

mt:VideoTrack
    a owl:Class;
    rdfs:subClassOf mt:MediaTrack;
    rdfs:comment "Contains a set of video clips organized in some sense." .

mt:AutomationTrack
    a owl:Class;
    rdfs:subClassOf mt:ProjectTrack;
    rdfs:comment "Represents a sequence of control parameters of some kind, or an envelope." .

mt:AnnotationTrack
    a owl:Class;
    rdfs:subClassOf mt:ProjectTrack;
    rdfs:comment "A sequence of labels or descriptors related to a signal. As an example, it may contain a sequence of FeatureEvents described in the audio feature ontology, or a label stating that someone kicked a microphone stand and a resulting artifact needs to be removed from the recording." .

mt:MidiTrack
    a owl:Class;
    rdfs:subClassOf mt:ProjectTrack;
    rdfs:comment "Container for a set of commands or events compatible with the MIDI specification." .

mt:MediaClip
    a owl:Class;
    rdfs:subClassOf event:Event;
    rdfs:comment """Represents a take of a usually short performance as stored in a media editor application. 
It is distinct from the signal itself, (e.g. a picture of a waveform on screen and its zoom ratio) and may not be directly related to a signal at all. A non-destructive editor is a good example of this concept. Generally we refer to an internal state of an editor as a result of a performance and a corresponding recording event.
			""" .

mt:AudioClip
    a owl:Class;
    rdfs:subClassOf mt:MediaClip;
    rdfs:comment """A type of MediaClip for Audio content. It may or may not form a musically meaningful section or part of a song. 
			""" .

mt:VideoClip
    a owl:Class;
    rdfs:subClassOf mt:MediaClip;
    rdfs:comment """Represents a sequence of images constituting a short section of video in a track.  
			""" .

mt:Annotation
    a owl:Class;
    rdfs:subClassOf event:Event;
    rdfs:comment """A label, marker or some sort of visualization associated with an event in a signal. 
			""" .

mt:AutomationEvent
    a owl:Class;
    rdfs:subClassOf event:Event;
    rdfs:comment """Reference to some parameter change, e.g. a volume change command in an automation track. 
			""" .

mt:Envelope
    a owl:Class;
    rdfs:comment """A continuous time function of some sort controlling one or more parameters. 
			""" .

mt:MIDICommand
    a owl:Class;
    rdfs:comment """Reference to a single MIDI message containing a command or event. (Clarify this from MIDI specs.) 
			""" .

mt:AutomationParameter
    a owl:Class;
    rdfs:comment """A numerical parameter used for automation, e.g. volume change. 
			""" .

foaf:Project
    a owl:Class .

foaf:Document
    a owl:Class .

event:Event
    a owl:Class .

mt:track
    a owl:ObjectProperty, owl11:AntisymmetricProperty;
    rdfs:domain mt:MultitrackProject;
    rdfs:comment "Used for specifying a track in a project.";
    rdfs:range mt:ProjectTrack .

mt:inProject
    a owl:ObjectProperty, owl11:AntisymmetricProperty;
    owl:inverseOf mt:track;
    rdfs:comment "Used for a track included in several projects. (inverse of hasTrack)." .

mt:clip
    a owl:ObjectProperty, owl11:AntisymmetricProperty;
    rdfs:domain mt:MediaTrack;
    rdfs:comment "a track contains a clip";
    rdfs:range mt:MediaClip .

mt:inTrack
    a owl:ObjectProperty, owl11:AntisymmetricProperty;
    owl:inverseOf mt:clip;
    rdfs:comment "Used for a clip included in several tracks. (inverse of holdsClip). " .

mt:annotation
    a owl:ObjectProperty, owl11:AntisymmetricProperty;
    rdfs:domain mt:AnnotationTrack;
    rdfs:comment "Relates an annotation track to an annotation.";
    rdfs:range mt:Annotation .

mt:automationEvent
    a owl:ObjectProperty, owl11:AntisymmetricProperty;
    rdfs:domain mt:AutomationTrack;
    rdfs:comment "Relates an automation track to a automation event.";
    rdfs:range mt:AutomationEvent .

mt:parameter
    a owl:ObjectProperty, owl11:AntisymmetricProperty;
    rdfs:domain mt:AutomationEvent;
    rdfs:comment "Used to link an automation event to a set of parameters. ";
    rdfs:range mt:AutomationParameter .

mt:envelope
    a owl:ObjectProperty, owl11:AntisymmetricProperty;
    rdfs:domain mt:AutomationTrack;
    rdfs:comment "Link an envelope to an automation track.";
    rdfs:range mt:Envelope .

mt:midiCommand
    a owl:ObjectProperty, owl11:AntisymmetricProperty;
    rdfs:domain mt:MidiTrack;
    rdfs:comment "Link a MIDI command to a MIDI Track.";
    rdfs:range mt:MIDICommand .

mt:representationOf
    a owl:ObjectProperty, owl11:AntisymmetricProperty;
    rdfs:domain mt:AudioClip;
    rdfs:comment "Relates an audio clip to a performance. ";
    rdfs:range mo:Performance .

mt:signal
    a owl:ObjectProperty, owl11:AntisymmetricProperty;
    rdfs:domain mt:MediaClip;
    rdfs:comment "A shortcut to relate a clip to a signal.";
    rdfs:range mo:Signal .

mo:Performance
    a owl:Class .

mo:Recording
    a owl:Class .

mo:Signal
    a owl:Class .

mt:value
    a owl:DatatypeProperty;
    rdfs:domain mt:AutomationParameter;
    rdfs:range xsd:float, xsd:integer, xsd:int .

mt:label
    a owl:DatatypeProperty;
    rdfs:domain mt:Annotation;
    rdfs:range xsd:string .

mt:functionOf
    a owl:DatatypeProperty;
    rdfs:domain mt:Envelope;
    rdfs:range xsd:string;
    rdfs:comment "A mathematical expression. Primarily for calculating a parameter between two automation events (e.g. can be a linear function of time.)" .

